examples/riscv/incr/incr_prop_transfScript.sml
@@ -1,0 +1,103 @@
+open HolKernel boolLib Parse bossLib;
+
+open markerTheory;
+
+open bir_programSyntax bir_program_labelsTheory;
+open bir_immTheory bir_valuesTheory bir_expTheory;
+open bir_tsTheory bir_bool_expTheory bir_programTheory;
+
+open bir_riscv_backlifterTheory;
+open bir_backlifterLib;
+open bir_compositionLib;
+
+open bir_lifting_machinesTheory;
+open bir_typing_expTheory;
+open bir_htTheory;
+
+open tutorial_smtSupportLib;
+
+open total_program_logicTheory;
+open total_ext_program_logicTheory;
+
+open jgmt_rel_bir_contTheory;
+
+open pred_setTheory;
+
+open program_logicSimps;
+
+open bir_env_oldTheory;
+open bir_program_varsTheory;
+
+open incrTheory;
+open incr_propTheory;
+open incr_symb_transfTheory;
+
+val birs_state_ss = rewrites (type_rws ``:birs_state_t``);
+
+val _ = new_theory "incr_prop_transf";
+
+val bprog_tm = (fst o dest_eq o concl) bir_incr_prog_def;
+
+Theorem bir_cont_incr_tm[local]:
+ bir_cont ^bprog_tm bir_exp_true (BL_Address (Imm64 0w))
+  {BL_Address (Imm64 4w)} {} (bir_incr_pre pre_x10)
+  (\l. if l = BL_Address (Imm64 4w) then (bir_incr_post pre_x10) else bir_exp_false)
+Proof
+ `{BL_Address (Imm64 4w)} <> {}` by fs [] >>
+ MP_TAC ((Q.SPECL [
+  `BL_Address (Imm64 0w)`,
+  `{BL_Address (Imm64 4w)}`,
+  `bir_incr_pre pre_x10`,
+  `\l. if l = BL_Address (Imm64 4w) then (bir_incr_post pre_x10) else bir_exp_false`
+ ] o SPEC bprog_tm o INST_TYPE [Type.alpha |-> Type`:'observation_type`]) abstract_jgmt_rel_bir_cont) >>
+ rw [] >>
+ METIS_TAC [abstract_jgmt_rel_incr]
+QED
+
+Theorem bir_cont_incr:
+ bir_cont bir_incr_prog bir_exp_true (BL_Address (Imm64 0w))
+  {BL_Address (Imm64 4w)} {} (bir_incr_pre pre_x10)
+   (\l. if l = BL_Address (Imm64 4w) then (bir_incr_post pre_x10)
+        else bir_exp_false)
+Proof
+ rw [bir_incr_prog_def,bir_cont_incr_tm]
+QED
+
+(* ---------------------------------- *)
+(* Backlifting BIR contract to RISC-V *)
+(* ---------------------------------- *)
+
+val riscv_cont_incr_thm =
+ get_riscv_contract_sing
+  bir_cont_incr
+  ``bir_incr_progbin``
+  ``riscv_incr_pre pre_x10`` ``riscv_incr_post pre_x10`` bir_incr_prog_def
+  [bir_incr_pre_def]
+  bir_incr_pre_def incr_riscv_pre_imp_bir_pre_thm
+  [bir_incr_post_def] incr_riscv_post_imp_bir_post_thm
+  bir_incr_riscv_lift_THM;
+
+Theorem riscv_cont_incr:
+ riscv_cont bir_incr_progbin 0w {4w} (riscv_incr_pre pre_x10) (riscv_incr_post pre_x10)
+Proof
+ ACCEPT_TAC riscv_cont_incr_thm
+QED
+
+(* unfolded theorem *)
+val birs_state_ss = rewrites (type_rws ``:birs_state_t``);
+val tm = concl riscv_cont_incr;
+val sset = std_ss++bir_wm_SS++bir_lifting_machinesLib.bmr_ss;
+val thms = [riscv_cont_def, t_jgmt_def, riscv_ts_def, riscv_weak_trs_def, riscv_incr_pre_def, riscv_incr_post_def, riscv_bmr_def, riscv_state_is_OK_def];
+(*
+EVAL tm;
+SIMP_CONV sset thms tm
+REWRITE_CONV  tm;
+*)
+val readable_thm = computeLib.RESTR_EVAL_CONV [``riscv_weak_trs``] tm;
+Theorem riscv_incr:
+  !pre_x10. ^((snd o dest_eq o concl) readable_thm)
+Proof
+  METIS_TAC [riscv_cont_incr, readable_thm]
+QED
+
+val _ = export_theory ();
