examples/riscv/incr/incr_symb_transfScript.sml
@@ -1,0 +1,443 @@
+open HolKernel boolLib Parse bossLib;
+
+open markerTheory;
+
+open distribute_generic_stuffLib;
+
+open bir_programSyntax bir_program_labelsTheory;
+open bir_immTheory bir_valuesTheory bir_expTheory;
+open bir_tsTheory bir_bool_expTheory bir_programTheory;
+
+open bir_riscv_backlifterTheory;
+open bir_backlifterLib;
+open bir_compositionLib;
+
+open bir_lifting_machinesTheory;
+open bir_typing_expTheory;
+open bir_htTheory;
+
+open tutorial_smtSupportLib;
+
+open bir_symbTheory birs_auxTheory;
+open HolBACoreSimps;
+open bir_program_transfTheory;
+
+open total_program_logicTheory;
+open total_ext_program_logicTheory;
+open symb_prop_transferTheory;
+
+open jgmt_rel_bir_contTheory;
+
+open bir_symbTheory;
+open birs_stepLib;
+open bir_symb_sound_coreTheory;
+open symb_recordTheory;
+open symb_interpretTheory;
+
+open pred_setTheory;
+
+open program_logicSimps;
+
+open bir_env_oldTheory;
+open bir_program_varsTheory;
+
+open incrTheory;
+open incr_propTheory;
+open incr_symb_execTheory;
+
+open distribute_generic_stuffTheory;
+
+val birs_state_ss = rewrites (type_rws ``:birs_state_t``);
+
+val _ = new_theory "incr_symb_transf";
+
+
+val bir_incr_pre = ``bir_incr_pre``;
+val bir_incr_post = ``bir_incr_post``;
+
+
+(* ------------------------------- *)
+(* BIR symbolic execution analysis *)
+(* ------------------------------- *)
+
+val (sys_i, L_s, Pi_f) = (symb_sound_struct_get_sysLPi_fun o concl) incr_symb_analysis_thm;
+
+Definition incr_analysis_L_def:
+ incr_analysis_L = ^(L_s)
+End
+
+val birs_state_init_lbl = ``<|bpc_label := BL_Address (Imm64 0w); bpc_index := 0|>``;
+val birs_state_end_lbl = (snd o dest_eq o concl o EVAL) ``bir_block_pc (BL_Address (Imm64 4w))``;
+
+Theorem incr_analysis_L_NOTIN_thm[local]:
+  (^birs_state_end_lbl) NOTIN incr_analysis_L
+Proof
+  EVAL_TAC
+QED
+
+(* ........................... *)
+(* ........................... *)
+(* ........................... *)
+
+val birs_state_init_pre = ``birs_state_init_pre_GEN ^birs_state_init_lbl incr_birenvtyl (mk_bsysprecond (bir_incr_pre pre_x10) incr_birenvtyl)``;
+
+Theorem birs_state_init_pre_EQ_thm:
+  ^((snd o dest_comb) sys_i) = ^birs_state_init_pre
+Proof
+  REWRITE_TAC [birs_state_init_pre_GEN_def, mk_bsysprecond_def, incr_bsysprecond_thm] >>
+  CONV_TAC (computeLib.RESTR_EVAL_CONV [``birs_eval_exp``] THENC birs_stepLib.birs_eval_exp_CONV)
+QED
+
+val incr_analysis_thm =
+  REWRITE_RULE [birs_state_init_pre_EQ_thm, GSYM bir_incr_prog_def] incr_symb_analysis_thm;
+
+Theorem incr_birenvtyl_EVAL_thm =
+ (REWRITE_CONV [incr_birenvtyl_def,
+   bir_lifting_machinesTheory.riscv_bmr_vars_EVAL,
+   bir_lifting_machinesTheory.riscv_bmr_temp_vars_EVAL] THENC EVAL)
+ ``incr_birenvtyl``;
+
+val birs_state_thm = REWRITE_CONV [incr_birenvtyl_EVAL_thm] birs_state_init_pre;
+
+(* ------ *)
+
+(* now the transfer *)
+
+val bprog_tm = (fst o dest_eq o concl) bir_incr_prog_def;
+
+val birs_symb_symbols_f_sound_prog_thm =
+  (SPEC (inst [Type`:'observation_type` |-> Type.alpha] bprog_tm) bir_symb_soundTheory.birs_symb_symbols_f_sound_thm);
+
+val birs_prop_transfer_thm =
+  (MATCH_MP symb_prop_transferTheory.symb_prop_transfer_thm birs_symb_symbols_f_sound_prog_thm);
+
+Definition bprog_P_def:
+  bprog_P x = P_bircont incr_birenvtyl (^bir_incr_pre x)
+End
+
+Definition bprog_Q_def:
+  bprog_Q x = Q_bircont (^birs_state_end_lbl) (set incr_prog_vars) (^bir_incr_post x)
+End
+
+Definition pre_bir_nL_def:
+  pre_bir_nL x = pre_bircont_nL incr_birenvtyl (^bir_incr_pre x)
+End
+
+Definition post_bir_nL_def:
+  post_bir_nL x = post_bircont_nL (^birs_state_end_lbl) (set incr_prog_vars) (^bir_incr_post x)
+End
+(* ........................... *)
+
+(* P is generic enough *)
+(* taken from "bir_exp_to_wordsLib" *)
+val type_of_bir_exp_thms =
+    let
+      open bir_immTheory
+      open bir_valuesTheory
+      open bir_envTheory
+      open bir_exp_memTheory
+      open bir_bool_expTheory
+      open bir_extra_expsTheory
+      open bir_nzcv_expTheory
+      open bir_interval_expTheory
+      in [
+        type_of_bir_exp_def,
+        bir_var_type_def,
+        bir_type_is_Imm_def,
+        type_of_bir_imm_def,
+        BExp_Aligned_type_of,
+        BExp_unchanged_mem_interval_distinct_type_of,
+        bir_number_of_mem_splits_REWRS,
+        BType_Bool_def,
+        bir_exp_true_def,
+        bir_exp_false_def,
+        BExp_MSB_type_of,
+        BExp_nzcv_ADD_DEFS,
+        BExp_nzcv_SUB_DEFS,
+        n2bs_def,
+        BExp_word_bit_def,
+        BExp_Align_type_of,
+        BExp_ror_type_of,
+        BExp_LSB_type_of,
+        BExp_word_bit_exp_type_of,
+        BExp_ADD_WITH_CARRY_type_of,
+        BExp_word_reverse_type_of,
+        BExp_ror_exp_type_of
+      ] end;
+
+Theorem bprog_P_entails_thm[local]:
+  P_entails_an_interpret (bir_symb_rec_sbir ^bprog_tm) (bprog_P pre_x10) (birs_symb_to_symbst ^birs_state_init_pre)
+Proof
+  ASSUME_TAC (GSYM incr_prog_vars_thm) >>
+  `incr_prog_vars = MAP PairToBVar incr_birenvtyl` by (
+    SIMP_TAC std_ss [incr_birenvtyl_def, listTheory.MAP_MAP_o, PairToBVar_BVarToPair_I_thm, listTheory.MAP_ID]
+  ) >>
+  POP_ASSUM (fn thm => FULL_SIMP_TAC std_ss [thm]) >>
+  IMP_RES_TAC (SIMP_RULE std_ss [] P_bircont_entails_thm) >>
+
+  SIMP_TAC std_ss [bprog_P_def] >>
+  POP_ASSUM (ASSUME_TAC o Q.SPEC `bir_incr_pre pre_x10`) >>
+  `bir_vars_of_exp (bir_incr_pre pre_x10) SUBSET set (MAP PairToBVar incr_birenvtyl)` by (
+    PAT_X_ASSUM ``A = set B`` (fn thm => REWRITE_TAC [GSYM thm]) >>
+    SIMP_TAC (std_ss++holBACore_ss) [bir_incr_pre_def, bir_incr_pre_def] >>
+    SIMP_TAC (std_ss++pred_setLib.PRED_SET_ss) [GSYM incr_prog_vars_thm, incr_prog_vars_def, bir_incr_pre_def] >>
+    SIMP_TAC (std_ss++pred_setLib.PRED_SET_ss++holBACore_ss) [listTheory.MEM, pred_setTheory.IN_INSERT]
+  ) >>
+  POP_ASSUM (fn thm => FULL_SIMP_TAC std_ss [thm]) >>
+  `ALL_DISTINCT (MAP FST incr_birenvtyl)` by (
+    SIMP_TAC (std_ss++listSimps.LIST_ss) [incr_birenvtyl_EVAL_thm]
+  ) >>
+  POP_ASSUM (fn thm => FULL_SIMP_TAC std_ss [thm]) >>
+  `IS_SOME (type_of_bir_exp (bir_incr_pre pre_x10))` by (
+    SIMP_TAC std_ss [bir_incr_pre_def, bir_incr_pre_def] >>
+    CONV_TAC (RAND_CONV (SIMP_CONV (srw_ss()) type_of_bir_exp_thms)) >>
+    SIMP_TAC (std_ss++holBACore_ss) [optionTheory.option_CLAUSES]
+  ) >>
+  POP_ASSUM (fn thm => FULL_SIMP_TAC std_ss [thm])
+QED
+
+(* ........................... *)
+(* ........................... *)
+(* ........................... *)
+
+(* ........................... *)
+(* proof for each end state individually: *)
+
+val sys1 = (snd o dest_eq o concl o REWRITE_CONV [incr_bsysprecond_thm]) birs_state_init_pre;
+val (Pi_func, Pi_set) = dest_comb Pi_f;
+(* Pi_func should be exactly ``IMAGE birs_symb_to_symbst`` *)
+val sys2s = pred_setSyntax.strip_set Pi_set;
+
+(*
+val sys2 = hd sys2s;
+*)
+val strongpostcond_goals = List.map (fn sys2 => ``
+    sys1 = ^sys1 ==>
+    sys2 = ^sys2 ==>
+    birs_symb_matchstate sys1 H' bs ==>
+    bir_eval_exp (^bir_incr_pre pre_x10) bs.bst_environ = SOME bir_val_true ==>
+    birs_symb_matchstate sys2 H' bs' ==>
+    bir_eval_exp (^bir_incr_post pre_x10) bs'.bst_environ = SOME bir_val_true
+  ``) sys2s;
+
+(* FIXME: this is implicitly proven already in bir_envTheory.bir_env_read_def *)
+Theorem bir_eval_precond_lookup_pre_x10_incr_thm:
+!x env.
+  bir_eval_exp (bir_incr_pre x) env = SOME bir_val_true ==>
+  bir_env_lookup "x10" env = SOME (BVal_Imm (Imm64 x))
+Proof
+ rw [bir_incr_pre_def] >>
+ Cases_on `env` >>
+ FULL_SIMP_TAC (std_ss++holBACore_ss) [
+  bir_envTheory.bir_env_lookup_type_def,
+  bir_envTheory.bir_env_read_def,
+  bir_envTheory.bir_env_check_type_def,
+  bir_envTheory.bir_env_lookup_def,bir_eval_exp_def,bir_eval_bin_pred_def
+ ] >>
+ Q.ABBREV_TAC `g = ?z. f "x10" = SOME z /\ BType_Imm Bit64 = type_of_bir_val z` >>
+ Cases_on `g` >-
+  (FULL_SIMP_TAC (std_ss++holBACore_ss) [bir_eval_bin_pred_def] >>
+   fs [Abbrev_def] >>
+   Cases_on `z` >> fs [type_of_bir_val_def] >>
+   FULL_SIMP_TAC (std_ss++holBACore_ss) [bir_eval_bin_pred_def,bir_immTheory.bool2b_def,bir_val_true_def] >>
+   FULL_SIMP_TAC (std_ss++holBACore_ss) [bool2w_def] >>
+   Q.ABBREV_TAC `bb = bir_bin_pred BIExp_Equal b (Imm64 x)` >>
+   Cases_on `bb` >> fs [] >>
+   FULL_SIMP_TAC (std_ss++holBACore_ss) [bir_exp_immTheory.bir_bin_pred_Equal_REWR]) >>
+ FULL_SIMP_TAC (std_ss++holBACore_ss) []
+QED
+
+(*
+val goal = hd strongpostcond_goals;
+*)
+val strongpostcond_thms = List.map (fn goal =>
+  prove(``^goal``,
+    (* birs_strongpostcond_impl_TAC *)
+    REPEAT STRIP_TAC >>
+    (* symbsof sys1 and sys2 IN symb_interpr_dom H' *)
+    `(birs_symb_symbols sys1 UNION birs_symb_symbols sys2) SUBSET symb_interpr_dom H'` by (
+      FULL_SIMP_TAC (std_ss) [UNION_SUBSET, birs_symb_matchstate_def, symb_interpr_for_symbs_def]
+    ) >>
+    FULL_SIMP_TAC (std_ss) [UNION_SUBSET] >>
+
+    (* get stuff out of bpre, then through matchstate *)
+    (* get stuff out of sys1 (environment and pcond) *)
+    (* get all of this through matchstate with sys2 to bs' *)
+    (* also get from sys2 through matchstate *)
+
+(*
+matchstate ==> know about concrete state from symbolic state info (pcond holds, symbolic values for state variables)
+matchstate of post state can use same interpretation
+precondition bprog also holds in bs
+*)
+
+    (* TODO: the following is still hard coded for the example *)
+
+    (* BVar "sy_x10" (BType_Imm Bit64) IN symbsof sys1 *)
+    `BVar "sy_x10" (BType_Imm Bit64) IN birs_symb_symbols sys1` by (
+      ASM_REWRITE_TAC [] >>
+      CONV_TAC (
+          REWRITE_CONV [birs_state_init_pre_GEN_def, incr_bsysprecond_thm] THENC
+          REWRITE_CONV [birenvtyl_EVAL_thm] THENC
+          computeLib.RESTR_EVAL_CONV [``birs_symb_symbols``] THENC
+          aux_setLib.birs_symb_symbols_MATCH_CONV THENC
+          EVAL
+        )
+    ) >>
+    (* the property (here: pre_x10 + 1) *)
+    `bir_env_lookup "x10" bs'.bst_environ = SOME (BVal_Imm (Imm64 (pre_x10 + 1w)))` by (
+      `BVar "sy_x10" (BType_Imm Bit64) IN symb_interpr_dom H'` by (
+        METIS_TAC [SUBSET_DEF]
+      ) >>
+
+      (* use bprog_P, but can also use the path condition in the end *)
+      `symb_interpr_get H' (BVar "sy_x10" (BType_Imm Bit64)) = SOME (BVal_Imm (Imm64 pre_x10))` by (
+        `bir_env_lookup "x10" bs.bst_environ = SOME (BVal_Imm (Imm64 pre_x10))` by (
+          METIS_TAC [bir_eval_precond_lookup_pre_x10_incr_thm]
+        ) >>
+
+        PAT_X_ASSUM ``A = ^sys1`` (fn thm => FULL_SIMP_TAC std_ss [thm]) >>
+        FULL_SIMP_TAC (std_ss++birs_state_ss) [birs_symb_matchstate_def] >>
+
+        FULL_SIMP_TAC (std_ss++birs_state_ss) [birs_matchenv_def, birs_interpret_fun_thm] >>
+        REPEAT (PAT_X_ASSUM ``!A.B`` (ASSUME_TAC o EVAL_RULE o Q.SPEC `"x10"`)) >>
+        FULL_SIMP_TAC (std_ss) [] >>
+        REV_FULL_SIMP_TAC (std_ss) [birs_interpret_fun_ALT_def, birs_interpret_get_var_def]
+      ) >>
+
+      (* now go through sys2 with matchstate to show that the increment holds in bs' *)
+      PAT_X_ASSUM ``A = (B:birs_state_t)`` (fn thm => FULL_SIMP_TAC std_ss [thm]) >>
+      FULL_SIMP_TAC (std_ss++birs_state_ss) [birs_symb_matchstate_def] >>
+      REPEAT (PAT_X_ASSUM ``!A.B`` (ASSUME_TAC o EVAL_RULE o Q.SPEC `"x10"`)) >>
+      FULL_SIMP_TAC (std_ss) [] >>
+
+      FULL_SIMP_TAC (std_ss++birs_state_ss) [birs_matchenv_def, birs_interpret_fun_thm] >>
+      REPEAT (PAT_X_ASSUM ``!A.B`` (ASSUME_TAC o EVAL_RULE o Q.SPEC `"x10"`)) >>
+      FULL_SIMP_TAC (std_ss) [] >>
+      REV_FULL_SIMP_TAC (std_ss) [birs_interpret_fun_ALT_def, birs_interpret_get_var_def] >>
+      FULL_SIMP_TAC (std_ss++holBACore_ss) []
+    ) >>
+
+    ASM_SIMP_TAC (std_ss++holBACore_ss) [bir_incr_post_def, bir_eval_bin_pred_def, bir_envTheory.bir_env_read_def, bir_envTheory.bir_env_check_type_def, bir_envTheory.bir_env_lookup_type_def] >>
+    EVAL_TAC
+  )
+) strongpostcond_goals;
+
+(*
+val sys2 = hd sys2s;
+*)
+val Pi_thms = List.map (fn sys2 =>
+  prove(``
+    sys1 = ^sys1 ==>
+    sys2 = ^sys2 ==>
+    birs_symb_matchstate sys1 H bs ==>
+    bprog_P pre_x10 (birs_symb_to_concst bs) ==>
+    symb_interpr_ext H' H ==>
+    birs_symb_matchstate sys2 H' bs' ==>
+    bprog_Q pre_x10 (birs_symb_to_concst bs) (birs_symb_to_concst bs')
+  ``,
+    REWRITE_TAC [bprog_P_def, bprog_Q_def] >>
+    REPEAT STRIP_TAC >>
+    Q_bircont_SOLVE3CONJS_TAC incr_prog_vars_thm >>
+
+    `birs_symb_matchstate sys1 H' bs` by (
+      METIS_TAC [bir_symb_soundTheory.birs_symb_matchstate_interpr_ext_IMP_matchstate_thm]
+    ) >>
+    FULL_SIMP_TAC std_ss [P_bircont_thm] >>
+    METIS_TAC strongpostcond_thms
+  )
+) sys2s;
+
+(* ........................... *)
+
+(* Q is implied by sys and Pi *)
+Theorem bprog_Pi_overapprox_Q_thm[local]:
+  Pi_overapprox_Q (bir_symb_rec_sbir ^bprog_tm) (bprog_P pre_x10) (birs_symb_to_symbst ^birs_state_init_pre) ^Pi_f(*(IMAGE birs_symb_to_symbst {a;b;c;d})*) (bprog_Q pre_x10)
+Proof
+  REWRITE_TAC [bir_prop_transferTheory.bir_Pi_overapprox_Q_thm, incr_bsysprecond_thm] >>
+  REPEAT GEN_TAC >>
+
+  REWRITE_TAC [pred_setTheory.IMAGE_INSERT, pred_setTheory.IMAGE_EMPTY, pred_setTheory.IN_INSERT, pred_setTheory.NOT_IN_EMPTY] >>
+  REPEAT STRIP_TAC >> (
+    FULL_SIMP_TAC std_ss [] >>
+    METIS_TAC Pi_thms
+  )
+QED
+(* ........................... *)
+
+(* apply the theorem for property transfer *)
+val bprog_prop_holds_thm =
+  SIMP_RULE (std_ss++birs_state_ss)
+    [birs_state_init_pre_GEN_def, birs_symb_symbst_pc_thm, GSYM incr_analysis_L_def] (
+  MATCH_MP
+    (MATCH_MP
+      (MATCH_MP
+         birs_prop_transfer_thm
+         bprog_P_entails_thm)
+      bprog_Pi_overapprox_Q_thm)
+    incr_analysis_thm);
+
+(* ........................... *)
+(* ........................... *)
+(* ........................... *)
+
+Theorem bir_abstract_jgmt_rel_incr_thm[local] =
+  REWRITE_RULE [GSYM post_bir_nL_def, GSYM pre_bir_nL_def]
+    (MATCH_MP
+      (MATCH_MP prop_holds_TO_abstract_jgmt_rel_thm incr_analysis_L_NOTIN_thm)
+      (REWRITE_RULE [bprog_P_def, bprog_Q_def] bprog_prop_holds_thm));
+
+(* ........................... *)
+(* now manage the pre and postconditions into contract friendly "bir_exec_to_labels_triple_precond/postcond", need to change precondition to "bir_env_vars_are_initialised" for set of program variables *)
+
+
+(* ........................... *)
+(* ........................... *)
+(* ........................... *)
+
+
+Theorem abstract_jgmt_rel_incr:
+ abstract_jgmt_rel (bir_ts ^bprog_tm) (BL_Address (Imm64 0w)) {BL_Address (Imm64 4w)}
+  (\st. bir_exec_to_labels_triple_precond st (bir_incr_pre pre_x10) ^bprog_tm)
+  (\st st'. bir_exec_to_labels_triple_postcond st' (\l. if l = BL_Address (Imm64 4w) then (bir_incr_post pre_x10) else bir_exp_false) ^bprog_tm)
+Proof
+  MATCH_MP_TAC (REWRITE_RULE [boolTheory.AND_IMP_INTRO] abstract_jgmt_rel_bir_exec_to_labels_triple_thm) >>
+  SIMP_TAC std_ss [] >>
+  Q.EXISTS_TAC `incr_birenvtyl` >>
+
+  CONJ_TAC >- (
+    (* bpre subset *)
+    REWRITE_TAC [bir_incr_pre_def] >>
+    SIMP_TAC (std_ss++pred_setLib.PRED_SET_ss) [GSYM incr_prog_vars_thm, incr_prog_vars_def] >>
+    SIMP_TAC (std_ss++pred_setLib.PRED_SET_ss++holBACore_ss) [listTheory.MEM, pred_setTheory.IN_INSERT]
+  ) >>
+
+  CONJ_TAC >- (
+    (* bpost subset *)
+    REWRITE_TAC [bir_incr_post_def] >>
+    SIMP_TAC (std_ss++pred_setLib.PRED_SET_ss) [GSYM incr_prog_vars_thm, incr_prog_vars_def] >>
+    SIMP_TAC (std_ss++pred_setLib.PRED_SET_ss++holBACore_ss) [listTheory.MEM, pred_setTheory.IN_INSERT]
+  ) >>
+
+  CONJ_TAC >- (
+    (* bpost is bool *)
+    REWRITE_TAC [bir_incr_post_def] >>
+    SIMP_TAC (std_ss++holBACore_ss) [bir_is_bool_exp_REWRS, type_of_bir_exp_def]
+  ) >>
+
+  CONJ_TAC >- (
+    (* ALL_DISTINCT envtyl *)
+    SIMP_TAC (std_ss++listSimps.LIST_ss) [incr_birenvtyl_EVAL_thm]
+  ) >>
+
+  CONJ_TAC >- (
+    (* envtyl = vars_of_prog *)
+    REWRITE_TAC [GSYM incr_prog_vars_thm] >>
+    SIMP_TAC std_ss [incr_birenvtyl_def, listTheory.MAP_MAP_o, PairToBVar_BVarToPair_I_thm, listTheory.MAP_ID]
+  ) >>
+
+  METIS_TAC [bir_abstract_jgmt_rel_incr_thm, pre_bir_nL_def, post_bir_nL_def, incr_prog_vars_thm]
+QED
+
+
+val _ = export_theory ();
